generalized manifest-generator (to lists of Copland phrases), plus misc refactoring of client-server logic and prep for demos

src/Negotiation_Dec.v
@@ -277,6 +277,15 @@ Definition myPlc_manifest_update (p:Plc) (m:Manifest) : Manifest :=
               ac_policy := oldAcPol*) |} := m in
       (Build_Manifest p oldasps oldKnowsOf oldContext oldPolicy (*oldAcPol*)).
 
+Definition pubkeys_manifest_update (ps:list Plc) (m:Manifest) : Manifest := 
+        let '{| my_abstract_plc := oldMyPlc;
+                asps := oldasps; 
+                uuidPlcs := oldKnowsOf; 
+                pubKeyPlcs := _; 
+                policy := oldPolicy (*; 
+                ac_policy := oldAcPol*) |} := m in
+        (Build_Manifest oldMyPlc oldasps oldKnowsOf ps oldPolicy (*oldAcPol*)).
+
 Definition asp_manifest_update (a:ASP) (m:Manifest) : Manifest :=
   match a with 
   | ASPC _ _ params => 
@@ -308,20 +317,58 @@ Definition asp_manifest_generator (a:ASP) (p:Plc) (e:Environment) : Environment 
     end.
 
 
-Fixpoint manifest_generator' (t:Term) (p:Plc) (e:Environment) : Environment :=
+Fixpoint manifest_generator' (p:Plc) (t:Term) (e:Environment) : Environment :=
   match t with
   | asp a => asp_manifest_generator a p e
   | att q t' => 
       let e' := plc_manifest_generator p q e in 
-        manifest_generator' t' q e'
-  | lseq t1 t2 => manifest_generator' t2 p (manifest_generator' t1 p e)
-  | bseq _ t1 t2 => manifest_generator' t2 p (manifest_generator' t1 p e)
-  | bpar _ t1 t2 => manifest_generator' t2 p (manifest_generator' t1 p e)
+        manifest_generator' q t' e'
+  | lseq t1 t2 => manifest_generator' p t2 (manifest_generator' p t1 e)
+  | bseq _ t1 t2 => manifest_generator' p t2 (manifest_generator' p t1 e)
+  | bpar _ t1 t2 => manifest_generator' p t2 (manifest_generator' p t1 e)
+  end.
+
+Check List.fold_left.
+  (*
+  fold_left
+	 : forall A B : Type, (A -> B -> A) -> list B -> A -> A
+  *)
+Check List.fold_right.
+  (*
+    fold_right
+	 : forall A B : Type, (B -> A -> A) -> A -> list B -> A
+   *)
+
+Check List.map.
+   (* map
+    : forall A B : Type, (A -> B) -> list A -> list B
+    *)
+
+Check List.remove.
+Check List.count_occ.
+
+Definition plc_list : list Plc := [P0; P1; P2].
+
+Compute (List.count_occ eq_plc_dec plc_list P1 ).
+Check Nat.leb.
+Check negb.
+
+Fixpoint dedup_list (ps:list Plc) : list Plc := 
+  match ps with
+  | [] => ps
+  | (p::ps') =>
+    if (eqb (List.count_occ eq_plc_dec ps' p) O)
+    then (p::(dedup_list ps'))
+    else dedup_list ps'
   end.
 
 
+Definition manifest_generator_terms (p:Plc) (ts:list Term) : Environment :=
+  fold_right (manifest_generator' p) e_empty ts.
+
+
 Definition manifest_generator (t:Term) (p:Plc) : Environment :=
-  manifest_generator' t p e_empty.
+  manifest_generator' p t e_empty.
 
 
 Fixpoint places' (t:Term) (ls:list Plc) : list Plc :=
@@ -333,8 +380,25 @@ Fixpoint places' (t:Term) (ls:list Plc) : list Plc :=
   | bpar _ t1 t2 => places' t2 (places' t1 ls)
   end.
 
-Definition places (t:Term) (p:Plc) : list Plc := 
+Definition places (p:Plc) (t:Term): list Plc := 
   p :: (places' t []).
+
+  (*
+  Check List.fold_right.
+  *)
+  (*
+    fold_right
+	 : forall A B : Type, (B -> A -> A) -> A -> list B -> A
+   *)
+
+
+Definition places_terms' (ts: list Term) (p:Plc) : list (list Plc) :=
+  List.map (places p) ts.
+
+Definition places_terms (ts:list Term) (p:Plc) : list Plc :=
+  dedup_list (List.concat (places_terms' ts p)).
+
+
 
 
 Definition fromSome{A:Type} (v:option A) (a:A) : A :=
@@ -347,41 +411,40 @@ Definition get_manifest_env_default (e:Environment) (p:Plc) : Manifest :=
   let m' := fromSome (map_get e p) empty_Manifest in
     myPlc_manifest_update p m'.
 
-  Check List.map.
-  (* map
-	 : forall A B : Type, (A -> B) -> list A -> list B
-   *)
-
 Definition get_unique_manifests_env' (ps:list Plc) (e:Environment) : list Manifest :=
   List.map (get_manifest_env_default e) ps.
 
-Definition get_unique_manifests_env (t:Term) (p:Plc) (e:Environment) : list Manifest :=
-  let ps := places t p in
+Definition get_unique_manifests_env (ts: list Term) (p:Plc) (e:Environment) : list Manifest :=
+  let ps := places_terms ts p in
     get_unique_manifests_env' ps e.
 
-Definition get_final_manifests_env (t:Term) (p:Plc) (e:Environment) : list Manifest :=
-  let ms := get_unique_manifests_env t p e in 
-  List.map (knowsof_myPlc_manifest_update) ms.
+Definition get_final_manifests_env (ts:list Term) (p:Plc) (e:Environment) : list Manifest :=
+  let ms := get_unique_manifests_env ts p e in 
+  let ms' := List.map (knowsof_myPlc_manifest_update) ms in
+  List.map (pubkeys_manifest_update (places_terms ts p)) ms'.
 
-
+(*
 Definition man_gen_run (t:Term) (p:Plc) : Environment := manifest_generator t p.
+*)
+
+Definition man_gen_run (ts:list Term) (p:Plc) : Environment := manifest_generator_terms p ts.
 
 Definition environment_to_manifest_list (e:Environment) : list Manifest :=
   map_vals e.
 
-Definition demo_man_gen_run (t:Term) (p:Plc) : list Manifest := 
-  get_final_manifests_env t p (man_gen_run t p).
+Definition demo_man_gen_run (ts:list Term) (p:Plc) : list Manifest := 
+  get_final_manifests_env ts p (man_gen_run ts p).
 
 
 
-Definition man_gen_res : Manifest := (fromSome (map_get (man_gen_run cert_style P0) P1) empty_Manifest).
+Definition man_gen_res : Manifest := (fromSome (map_get (man_gen_run [cert_style] P0) P1) empty_Manifest).
 Compute man_gen_res.
 
 Compute man_gen_run.
 
 
 (*
-Example mytest : (man_gen_run = map_empty).
+Example mytest : (man_gen_run [cert_style] P0 = map_empty).
 Proof.
   cbv.
   break_let.
@@ -395,7 +458,7 @@ Proof.
 *)
 
 
-Eval cbv iota in (fromSome (map_get (man_gen_run cert_style P0) P1) empty_Manifest).
+Eval cbv iota in (fromSome (map_get (man_gen_run [cert_style] P0) P1) empty_Manifest).
 
 
 
