src/Client_AM.v
@@ -22,33 +22,83 @@ Definition gen_authEvC_if_some (ot:option Term) (pFrom:Plc) : AM EvC :=
     ret (evc auth_rawev auth_et)
   | None => ret (evc [] mt)
   end.
-  
+
+  Print AM_Result.
 
 Definition am_sendReq_gen (t:Term) (pFrom:Plc) (pTo:Plc)
-           (initEv:option EvC) (authPhrase:option Term) (plcCb : CakeML_PlcCallback) : AM AppResultC :=
+  (initEv:option EvC) (authPhrase:option Term) 
+  (plcCb : CakeML_PlcCallback) (app_bool:bool) : AM AM_Result :=
+evcIn <- gen_nonce_if_none initEv ;;
+auth_evc <- gen_authEvC_if_some authPhrase pFrom  ;;
+let '(evc init_ev init_et) := evcIn in
+let targetUUID := plcCb pTo in
+let resev := am_sendReq t targetUUID auth_evc init_ev in 
+(*
+let resev := run_cvm_rawEv t pFrom init_ev in *)
+match app_bool with
+| true => 
+let expected_et := eval t pTo init_et in
+app_res <- gen_appraise_AM expected_et resev ;;
+ ret (am_appev app_res)
+| false => ret (am_rawev resev)
+end.
+  
+(*
+Definition am_sendReq_gen (t:Term) (pFrom:Plc) (pTo:Plc)
+           (initEv:option EvC) (authPhrase:option Term) 
+           (plcCb : CakeML_PlcCallback) (app_bool:bool) : AM AM_Result :=
   evcIn <- gen_nonce_if_none initEv ;;
   auth_evc <- gen_authEvC_if_some authPhrase pFrom  ;;
   let '(evc init_ev init_et) := evcIn in
   let targetUUID := plcCb pTo in
   let resev := am_sendReq t targetUUID auth_evc init_ev in
-  let expected_et := eval t pTo init_et in
-  gen_appraise_AM expected_et resev.
+    match app_bool with
+    | true => 
+        let expected_et := eval t pTo init_et in
+        app_res <- gen_appraise_AM expected_et resev ;;
+          ret (am_appev app_res)
+    | false => ret (am_rawev resev)
+    end.
+    *)
+
+Definition am_sendReq_dispatch (maybeAuthTerm : option Term) (nonceB:bool) (t : Term) 
+                               (source : Plc) (dest : Plc) (app_bool:bool)
+                               (plcCb : CakeML_PlcCallback) : AM AM_Result :=
+  let nonce_param := 
+    if(nonceB) 
+    then None 
+    else (Some (evc [] mt)) in
+    am_sendReq_gen t source dest nonce_param maybeAuthTerm plcCb app_bool.
 
 
+Definition am_sendReq_dispatch_default_auth (t : Term) (source : Plc) (dest : Plc) 
+    (plcCb : CakeML_PlcCallback) (auth : bool) (app_bool:bool) : AM AM_Result :=
+    let auth_term := (ssl_sig_parameterized source) in
+      let auth_param := 
+       if(auth)
+       then (Some auth_term)
+       else None in
+          am_sendReq_dispatch auth_param true t source dest app_bool plcCb.
+
+
+
+
+(*
 Definition am_sendReq_nonce (t:Term) (pFrom:Plc) (pTo:Plc) (plcCb : CakeML_PlcCallback) : AM AppResultC :=
   am_sendReq_gen t pFrom pTo None None plcCb.
+  *)
 
+(*
 Definition am_sendReq_nonce_auth (t:Term) (pFrom:Plc) (pTo:Plc) (plcCb : CakeML_PlcCallback): AM AppResultC :=
   let auth_phrase := (* kim_meas *) ssl_sig in
   am_sendReq_gen t pFrom pTo None (Some auth_phrase) plcCb.
+  *)
   
-Definition am_sendReq_auth (t:Term) (pFrom:Plc) (pTo:Plc) (initEv:RawEv) (plcCb : CakeML_PlcCallback) : AM AppResultC :=
+
+(*
+Definition am_sendReq_auth (t:Term) (pFrom:Plc) (pTo:Plc) (initEv:RawEv) 
+                           (plcCb : CakeML_PlcCallback) : AM AM_Result :=
   let auth_phrase := (* kim_meas *) ssl_sig in
   let initEv_et := mt in (* TODO:  make this a param? *)
   am_sendReq_gen t pFrom pTo (Some (evc initEv initEv_et)) (Some auth_phrase) plcCb.
-
-Definition am_sendReq_dispatch (auth : bool) (t : Term) (source : Plc) (dest : Plc) 
-    (plcCb : CakeML_PlcCallback) : AM AppResultC :=
-  if (auth)
-  then (am_sendReq_nonce_auth t source dest plcCb)
-  else (am_sendReq_nonce t source dest plcCb).
+*)
