src/IO_Stubs.v
@@ -55,3 +55,6 @@ Admitted.
 
 Definition appraise_auth_tok (res:AppResultC) : bool.
 Admitted.
+
+Definition print_auth_tok (tok:ReqAuthTok) : unit.
+Admitted.
